theories/SLOT.v
@@ -18,8 +18,8 @@ From SLOT Require Export
      Foundations
      Generator
      Commutativity
-     Tactics
-     Handlers.
+     Handlers
+     Bruteforce.
 
 From Coq Require Import List.
 Import ListNotations.
@@ -28,69 +28,3 @@ Import ListNotations.
 Require Handlers.Deterministic
         Handlers.Mutex.
 (* end: hide *)
-
-Module Example.
-  Import Handlers.Deterministic Handlers.Deterministic.Var Mutex.
-
-  Inductive handlerId := var | mutex.
-
-  Ltac2 handlerSpec () := ['(Var.t nat); 'Mutex.t].
-
-  Definition handler := ltac2:(makeClass handlerSpec).
-  Definition reqT := ltac2:(makeRequestType handlerSpec 'handlerId).
-  Definition req := ltac2:(makeReq handlerSpec 'handlerId 'reqT 'handler).
-  Definition stateG := ltac2:(makeStateGetter handlerSpec 'handler 'handlerId).
-
-  Definition Req := handler_request_t handler.
-  Definition Rep := handler_reply_t handler.
-
-  Definition prog : @Program Req Rep :=
-    do _ <- req mutex grab;
-    do x <- req var read;
-    do _ <- req var (write (x + 1));
-    done (req mutex release).
-
-  Import better_parallel.
-
-  Definition system := of_progs [prog; prog].
-
-  Lemma canned_par_opt_nil {last_pid}
-    {t : Trace Req Rep}
-    (H : Ensembles.In (GenEnsembleOpt {| last_pid := last_pid; processes := []|}) t) :
-    t = [].
-  Proof.
-    inversion H.
-    - reflexivity.
-    - inversion H0.
-    - inversion H0.
-  Qed.
-
-  Lemma canned_par_opt_two {last_pid p1 p2 rest}
-    {t : Trace Req Rep}
-    (H : Ensembles.In (GenEnsembleOpt {| last_pid := last_pid; processes := p1 :: p2 :: rest|}) t) :
-    exists pid1 req rep,
-      t = [pid1 @ rep <~ req].
-  Admitted.
-
-  Goal forall n,
-      -{{ fun s => stateG s var = n }} GenEnsembleOpt system {{ fun s => stateG s var = n + 2 }}.
-  Proof with auto with slot.
-    intros n.
-    unfold_ht.
-    unfold system, better_parallel.of_progs in Ht.
-    inversion Ht.
-    3:{ inversion Ht.
-        3:{
-      apply canned_par_opt_two in Ht.
-    specialize (canned_par_opt_two Ht) as H.
-
-
-    cbn in Ht.
-    inversion Ht.
-    - exfalso. simpl in H. firstorder; discriminate.
-    - simpl in H. firstorder.
-
-    apply parallel_processes_ht...
-    unfold_ht. inversion Ht.
-  Abort.
-End Example.
