theories/Bruteforce.v
@@ -1,0 +1,452 @@
+(** * SLOT model checker *)
+
+From SLOT Require Export
+     Foundations
+     Generator
+     Commutativity
+     Handlers.
+
+From Ltac2 Require Import Ltac2.
+Import Ltac2.Notations Ltac2.Printf.
+  (* Init List Ind Env Control Option Constr Std Array Notations Fresh Printf. *)
+
+From Coq Require Import List Lia.
+Import ListNotations.
+
+Import better_parallel.
+
+Section canned_lemmas.
+  Context `{Hhandler : IOHandler}.
+  Let TE := ProcessEvent (IOp Request Reply).
+
+  Lemma canned_par_opt_nil {last_pid}
+    (t : list TE)
+    (Hgen : GenEnsembleOpt {| last_pid := last_pid; processes := []|} t) :
+    t = [].
+  Proof.
+    inversion Hgen.
+    - reflexivity.
+    - inversion H.
+  Qed.
+
+  Lemma canned_par_opt_cons {last_pid : PID}
+    {p : @Runnable Request Reply}
+    {rest : list (@Runnable Request Reply)}
+    (t : list TE)
+    (Hgen : GenEnsembleOpt {| last_pid := last_pid; processes := p :: rest|} t) :
+    exists g' te t',
+      t = te :: t' /\
+        {| last_pid := last_pid; processes := p :: rest|} ~~> g' & te /\
+        can_follow_hd te t' /\
+        GenEnsembleOpt g' t'.
+  Admitted.
+End canned_lemmas.
+
+(** A tactic that tries to find a contradiction to [can_follow_hd] hypothesis named [hi].
+
+ pid_compare_tact is a tactic that finds evidence that [pid1 > pid2]
+
+ commut_tact is a tactic that finds evidence that trace elements commute. *)
+Ltac2 elim_by_comm0 pid_compare_tact commut_tact (hi : ident) :=
+  let hpid := Fresh.in_goal @Hpid in
+  let hnoncomm := Fresh.in_goal @Hnoncomm in
+  let hcomm := Fresh.in_goal @Hcomm in
+  let h := Control.hyp hi in
+  let try_find_comm () :=
+    lazy_match! Constr.type (Control.hyp hnoncomm) with
+    |  ~ events_commute ?a ?b => assert ($hcomm : events_commute $a $b) by commut_tact ()
+    end;
+    let h1 := Control.hyp hnoncomm in
+    let h2 := Control.hyp hcomm in
+    (destruct ($h1 $h2)) in
+  destruct $h as [$hpid|$hnoncomm] > [solve [ pid_compare_tact () ] | solve [ try_find_comm () ] ].
+
+Ltac2 elim_by_comm hi := elim_by_comm0
+                           (fun () => ltac1:(lia))
+                           (fun () => (first [apply compose_comm | apply compose_comm_rev]; auto with slot))
+                           hi.
+
+From SLOT Require Import Deterministic Mutex.
+
+Section tests.
+  Import Var.
+
+  Let Handler := compose (Var.t nat) (Var.t nat).
+  Let Req := handler_request_t Handler.
+  Let Rep := handler_reply_t Handler.
+
+  Goal forall t (rep1 rep2 : nat) , can_follow_hd (1 @ rep1 <~ inl read) [0 @ rep2 <~ inr read; t] -> False.
+  Proof.
+    intros.
+    elim_by_comm @H.
+  Qed.
+
+  Goal forall t (rep1 rep2 : nat) , can_follow_hd (1 @ rep1 <~ inr read) [0 @ rep2 <~ inl read; t] -> False.
+  Proof.
+    intros.
+    elim_by_comm @H.
+  Qed.
+
+  Goal forall rep1 rep2, can_follow_hd (1 @ rep1 <~ inl (write 1)) [0 @ rep2 <~ inr (write 1)] -> False.
+    intros.
+    elim_by_comm @H.
+  Qed.
+
+  Goal forall t (rep1 rep2 : nat) , can_follow_hd (1 @ rep1 <~ inl read) [0 @ rep2 <~ inl read; t] -> False.
+  Proof.
+    intros. (* TODO *)
+  Abort.
+
+  Goal forall t (rep1 rep2 : nat) , can_follow_hd (0 @ rep1 <~ inl read) [1 @ rep2 <~ inr read; t] -> False.
+  Proof.
+    intros.
+    Fail elim_by_comm @H.
+  Abort.
+
+  Goal forall t (rep1 : nat) , can_follow_hd (1 @ rep1 <~ inl read) [0 @ I <~ inl (write 1); t] -> False.
+  Proof.
+    intros.
+    Fail elim_by_comm @H.
+  Abort.
+
+
+End tests.
+
+(** Helper tactic to unfold nested [a /\ b /\ ...] or [a \/ b \/  ...] expressions *)
+Ltac2 rec split_all_clauses (n : ident) :=
+  let h := Control.hyp n in
+  lazy_match! Constr.type h with
+  | ?a \/ ?b => destruct $h as [$n | $n] > [() | split_all_clauses n]
+  | ?a /\ ?b =>
+      let f1 := Fresh.in_goal n in
+      destruct $h as [$f1 $n];
+      lazy_match! Constr.type (Control.hyp f1) with
+      | ?a = ?b => subst
+      | _ => ()
+      end;
+      try (split_all_clauses n)
+  | _ => ()
+  end.
+
+Section tests.
+    (* Test: *)
+  Goal True \/ True \/ True \/ True -> False.
+  Proof.
+    intros H.
+    split_all_clauses @H > [() | () | () | ()].
+  Abort.
+
+  Goal forall a b, True /\ a = 1 /\ b = 2 /\ a = b -> False.
+  Proof.
+    intros a b H.
+    split_all_clauses @H.
+  Abort.
+End tests.
+
+(** A helper tactic that simplifies the result of applying
+[canned_par_opt_two] lemma to a generator: *)
+Ltac2 simpl_par_cons_rep (n : ident) (g : ident) (te : ident) :=
+  let rep := Fresh.in_goal @rep in
+  let h := Control.hyp n in
+  destruct $h as [$rep $n];
+  let h := Control.hyp n in
+  let hte := Fresh.in_goal @Hte in
+  injection $h as $n $hte;
+  (* subst $g; *)
+  (* subst $te. *)
+  subst.
+
+Section tests.
+  Goal forall g te,
+      (exists rep : True, Some (g, te) = Some (1, 2)) ->
+      g = 1 /\ te = 2.
+  Proof.
+    intros g te H.
+    simpl_par_cons_rep @H @g @te.
+    split; reflexivity.
+  Qed.
+End tests.
+
+Local Ltac2 Type state := {comm_hyp : ident; te : ident; trace : ident; depth : int}.
+
+Ltac2 gen_par_step (handler_instance : constr) (t : ident) (gen_hyp_n : ident) :=
+  lazy_match! Constr.type (Control.hyp gen_hyp_n) with
+  | @GenEnsembleOpt (@Parallel ?req_t ?rep_t) ?state_t ?event_t ?state_space_inst ?generator_inst {| processes := [] |} _ =>
+      apply (@canned_par_opt_nil $req_t $rep_t) in $gen_hyp_n;
+      subst $t;
+      None
+  |  @GenEnsembleOpt (@Parallel ?req_t ?rep_t) ?state_t ?event_t ?state_space_inst ?generator_inst
+                     {| last_pid := ?pid; processes := ?pfirst :: ?prest |} ?t_hyp =>
+      let g' := Fresh.in_goal @g in
+      let te := Fresh.in_goal @te in
+      let t' := Fresh.in_goal @t' in
+      let ht := Fresh.in_goal @Ht in
+      let hcomm := Fresh.in_goal @Htete' in
+      let hg' := Fresh.in_goal @Hg' in
+      apply (@canned_par_opt_cons $req_t $rep_t $handler_instance $pid $pfirst $prest $t_hyp) in $gen_hyp_n;
+      let h := Control.hyp gen_hyp_n in
+      destruct $h as [$g' [$te [$t' [$ht [$gen_hyp_n [$hcomm $hg']]]]]];
+      (* subst $t; *)
+      Some (g', te, t', ht, hcomm, hg')
+  | ?invalid =>
+      let msg := fprintf "gen_par_step invalid argument %t" invalid in
+      Control.throw (Init.Tactic_failure (Some msg))
+  end.
+
+Section tests.
+  Let Handler := Var.t nat.
+  Let Req := handler_request_t Handler.
+  Let Rep := handler_reply_t Handler.
+
+  Let prog n : @Program Req Rep := done Var.write n.
+
+  Goal forall t, GenEnsembleOpt (of_progs []) t -> t = [].
+  Proof.
+    intros t Hg.
+    unfold of_progs in Hg.
+    gen_par_step 'Handler @t @Hg.
+    reflexivity.
+  Qed.
+
+  Goal forall t, GenEnsembleOpt (of_progs [prog 1]) t -> False.
+  Proof.
+    intros t Hg.
+    unfold of_progs, prog in Hg.
+    gen_par_step 'Handler @t @Hg > [()].
+  Abort.
+
+  Goal forall t, GenEnsembleOpt (of_progs [prog 1; prog 2]) t -> False.
+  Proof.
+    intros t Hg.
+    unfold of_progs, prog in Hg.
+    gen_par_step 'Handler @t @Hg > [()].
+  Abort.
+End tests.
+
+Ltac2 maybe_elim_by_comm (state : state option) cont :=
+  match state with
+  | None =>
+      cont ()
+  | Some {comm_hyp := h; depth := d} =>
+      (* printf "maybe elim by comm %i %I:%t" d h (Constr.type (Control.hyp h)); *)
+      Control.plus (fun () => elim_by_comm h) (fun _ => Control.enter cont)
+  end.
+
+Section tests.
+  Goal True -> True.
+    maybe_elim_by_comm None (fun () => constructor).
+  Qed.
+
+  Goal forall (rep1 rep2 : nat), can_follow_hd (1 @ rep1 <~ inl Var.read) [0 @ rep2 <~ inr Var.read] -> False.
+    intros.
+    maybe_elim_by_comm (Some {comm_hyp := @H; te := @unused; trace := @unused; depth := 1})
+      (fun () => fail).
+  Qed.
+
+  Goal forall (rep1 rep2 : True), can_follow_hd (1 @ rep1 <~ inl (Var.write 1)) [0 @ rep2 <~ inr (Var.write 1)] -> False.
+    intros.
+    maybe_elim_by_comm (Some {comm_hyp := @H; te := @unused; trace := @unused; depth := 1})
+      (fun () => fail).
+  Qed.
+End tests.
+
+Local Ltac2 inc_depth state :=
+  match state with
+  | None => 1
+  | Some {depth := d} =>
+      Int.add d 1
+  end.
+
+Ltac2 rec gen_par_unfold0 (handler_instance : constr) (t : ident) (gen_hyp_n : ident) (state0 : state option) post_hook :=
+  match gen_par_step handler_instance t gen_hyp_n with
+  | None =>
+      post_hook ()
+  | Some (g', te, t', ht, hcomm, hg') =>
+      cbn in $gen_hyp_n;
+      let state1 := Some {comm_hyp := hcomm; te := te; trace := t'; depth := inc_depth state0} in
+      split_all_clauses gen_hyp_n >
+        [simpl_par_cons_rep gen_hyp_n g' te;
+         (* NB: It's important that elim by comm tactic runs on a
+         [can_follow_hd] hypothesis generated _2_ steps before, since
+         it has to analyze 2 trace elements: *)
+         maybe_elim_by_comm state0
+           (fun () =>
+              post_hook () >
+                [gen_par_unfold0 handler_instance t' hg' state1 post_hook..])
+          ..]
+  end.
+
+Ltac2 gen_par_unfold (handler_instance : constr) (t : ident) (hyp_g : ident) hook :=
+  gen_par_unfold0 handler_instance t hyp_g None hook.
+
+Section tests.
+  Let Handler := Var.t nat.
+  Let Req := handler_request_t Handler.
+  Let Rep := handler_reply_t Handler.
+
+  Let P := @Program Req Rep.
+
+  Goal forall t, GenEnsembleOpt (of_progs []) t -> t = [].
+  Proof.
+    intros t Hg.
+    unfold of_progs in Hg.
+    gen_par_unfold 'Handler @t @Hg (fun _ => ()).
+    reflexivity.
+  Qed.
+
+  Goal forall t,
+      let p : P := done (Var.write 1) in
+      GenEnsembleOpt (of_progs [p]) t -> t = [0 @ I <~ Var.write 1].
+  Proof.
+    intros t p Hg. subst p.
+    unfold of_progs in Hg.
+    gen_par_unfold 'Handler @t @Hg (fun _ => ()).
+    destruct rep.
+    reflexivity.
+  Qed.
+
+  Goal forall t,
+      let pp : list P := [done (Var.write 1); done (Var.write 2)] in
+      GenEnsembleOpt (of_progs pp) t ->
+            t = [0 @ I <~ Var.write 1; 1 @ I <~ Var.write 2] \/
+              t = [1 @ I <~ Var.write 2; 0 @ I <~ Var.write 1].
+  Proof.
+    intros t pp Hg. subst pp.
+    unfold of_progs in Hg.
+    gen_par_unfold 'Handler @t @Hg (fun _ => ());
+      destruct rep; destruct rep0; subst.
+    - left. reflexivity.
+    - right. reflexivity.
+  Qed.
+
+  Goal forall t,
+      let p : P := do _ <- (Var.write 1); done (Var.write 2) in
+      GenEnsembleOpt (of_progs [p]) t ->
+            t = [0 @ I <~ Var.write 1; 0 @ I <~ Var.write 2].
+  Proof.
+    intros t p Hg. subst p.
+    unfold of_progs in Hg.
+    gen_par_unfold 'Handler @t @Hg (fun _ => ());
+      destruct rep; destruct rep0; subst.
+    - reflexivity.
+  Qed.
+
+  Let prog : P :=
+        do n <- Var.read;
+        done Var.write (n + 1).
+
+  Let system := of_progs [prog; prog].
+
+  Goal forall t, GenEnsembleOpt system t -> False.
+  Proof.
+    intros t Hg.
+    unfold system, of_progs, prog in Hg.
+    gen_par_unfold 'Handler @t @Hg (fun s => ()) > [() | () | () | () | () | ()].
+  Abort.
+
+  Let handler := compose (Var.t nat) (Var.t nat).
+
+  Goal forall t, GenEnsembleOpt (of_progs [done inl (Var.write 1); done inr (Var.write 2)]) t ->
+            t = [0 @ I <~ inl (Var.write 1); 1 @ I <~ inr (Var.write 2)].
+  Proof.
+    intros t H.
+    unfold of_progs in H.
+    gen_par_unfold 'handler @t @H (fun s => ()).
+    - destruct rep. destruct rep0. reflexivity.
+  Qed.
+End tests.
+
+Ltac2 handler_step (hypn : ident) : (ident * ident * ident) option :=
+  let h := Control.hyp hypn in
+  cbn in $hypn;
+  lazy_match! Constr.type h with
+  | ReachableByTrace _ [] _ =>
+      let s := Fresh.in_goal @s in
+      let hx := Fresh.in_goal @Hx in
+      let hy := Fresh.in_goal @Hy in
+      let hz := Fresh.in_goal @Hz in
+      inversion $h as [$s $hx $hy $hz | ];
+      subst; clear $hypn;
+      None
+  | ReachableByTrace _ (_ :: _) _ =>
+      let s' := Fresh.in_goal @s in
+      let te := Fresh.in_goal @te in
+      let tail := Fresh.in_goal @tail in
+      let hcr := Fresh.in_goal @Hcr in
+      let htl := Fresh.in_goal @Htl in
+      inversion_clear $h as [ |? $s' ? $te $tail $hcr $hypn];
+      cbn in $hcr;
+      Some (te, s', hcr)
+  end.
+
+Module Example.
+  Import Handlers.Deterministic Handlers.Deterministic.Var.
+
+  Inductive handlerId := var | mutex.
+
+  Ltac2 handlerSpec () := ['(Var.t nat); 'Mutex.t].
+
+  Definition handler := ltac2:(makeClass handlerSpec).
+  Definition reqT := ltac2:(makeRequestType handlerSpec 'handlerId).
+  Definition req := ltac2:(makeReq handlerSpec 'handlerId 'reqT 'handler).
+  Definition stateG := ltac2:(makeStateGetter handlerSpec 'handler 'handlerId).
+  Definition Req := handler_request_t handler.
+  Definition Rep := handler_reply_t handler.
+  Definition TE := ProcessEvent (@IOp Req Rep).
+
+  (* An example program where all syscalls commute: *)
+  Definition prog_inl : @Program Req Rep :=
+    do _ <- req var read;
+    done req var read.
+
+  Definition prog_inr : @Program Req Rep :=
+    do _ <- req mutex release;
+    done req mutex release.
+
+  Goal forall t,
+      GenEnsembleOpt (of_progs [prog_inl; prog_inr]) t ->
+      exists n1 n2 r1 r2,
+        t = [0 @ n1 <~ req var read; 0 @ n2 <~ req var read; 1 @ r1 <~ req mutex release; 1 @ r2 <~ req mutex release].
+  Proof.
+    intros t Hg.
+    unfold of_progs, prog_inl, prog_inr, req in Hg.
+    gen_par_unfold 'handler @t @Hg (fun _ => ()).
+    - exists rep. exists rep0. exists rep1. exists rep2.
+      reflexivity.
+  Qed.
+
+  Definition prog : @Program Req Rep :=
+    do _ <- req mutex grab;
+    do x <- req var read;
+    do _ <- req var (write (x + 1));
+    done (req mutex release).
+
+  Let system := of_progs [prog; prog].
+
+  Goal forall n,
+      -{{ fun s => stateG s var = n }}
+         GenEnsembleOpt system
+       {{ fun s => stateG s var = n + 2 }}.
+  Proof with auto with slot.
+    intros n t Hg [s_begin1 s_begin2] [s_end1 s_end2] Hrbt Hpre.
+    unfold stateG in *. simpl in *.
+    unfold Ensembles.In, system, of_progs, prog in Hg.
+    gen_par_unfold 'handler @t @Hg
+      (fun _ => match handler_step @Hrbt with
+             | None => ()
+             | Some (te, s, hcr) =>
+                 destruct s;
+                 unfold compose_state_transition in hcr;
+                 (* printf "%t" (type (hyp hcr)); *)
+                 (* ifcatch (fun () => split_all_clauses hcr) (fun _  => ()) (fun f => Message.print (Message.of_exn f)) *)
+                 split_all_clauses hcr;
+                 lazy_match! goal with
+                 | [ h : mutex_state_transition _ _ _  |- _] =>
+                     let h := Control.hyp h in
+                     inversion $h
+                 end
+             end).
+    - ltac1:(lia).
+    - ltac1:(lia).
+  Qed.
+End Example.
